timing/riscv/RISCVTiming.v
@@ -32,7 +32,7 @@ Module RISCVTiming (cpu : CPUTimingBehavior) (prog : ProgramInformation) <: Timi
 
     Definition lifted_prog := lift_riscv binary.
 
-    Definition cycles_per_instruction_at_addr (s : store) (a : addr) : N :=
+    Definition time_of_addr (s : store) (a : addr) : N :=
         let regvalue s r := if r =? 0 then 0 else s (rv_varid r) in
         let bop s time_inf rs1 rs2 op : N :=
             op (regvalue s rs1) (regvalue s rs2) in
